---
title: "Survival analysis note 2"
date: 2025-07-24
math: true
#categories: [test-category]
#tags: [test-tag]
---

# Survival Analysis: Parametric Distributions and Maximum Likelihood

These notes introduce the basics of using parametric models for survival data, and explain how to construct the likelihood function when data are censored.

---

## 1. Key Notations

- **Survival Function**:  
  $S(t; \theta) = \Pr(T_i > t)$  
  Probability that event time $T_i$ exceeds time $t$, given parameter $\theta$.

- **Censoring Distribution** (for right censoring):  
  $G(c) = \Pr(C_i < c)$  
  Probability that the censoring time $C_i$ is less than $c$.  
  *Alternate form:* $G(c^+) = \Pr(C_i > c)$.

- **Density Functions**:  
  - $f(t; \theta)$: density of event time  
  - $g(c)$: density of censoring time  

- **Complete vs Censored Observation**:  
  - $\delta_i = 1$: Event is observed  
  - $\delta_i = 0$: Event is censored  

---

## 2. Independence Assumption

- **Assume**: $T_i$ (event time) and $C_i$ (censoring time) are independent.

---

## 3. Likelihood Contributions

- For **subject $i$** with observed time $y_i$ and event indicator $\delta_i$:

  - If **event observed** ($\delta_i = 1$):  
    - Contribution to likelihood:  
      $P(T_i=y_i,C_i>y_i)=f(y_i; \theta) \cdot G(y_i^+)$

  - If **censored** ($\delta_i = 0$):  
    - Contribution to likelihood:  
      $P(C_i=y_i,T_i>y_i)=g(y_i) \cdot S(y_i; \theta)$

---

## 4. The Full Likelihood Function

Given $n$ subjects with data $(y_i, \delta_i)$:

\[
L = \prod_{i=1}^n (f(y_i; \theta) \cdot G(y_i^+))^{\delta_i}  (g(y_i) \cdot S(y_i; \theta))^{1-\delta_i} \,
\]

\[
= \prod_{i=1}^n (f(y_i; \theta)^{\delta_i} S(y_i; \theta)^{1-\delta_i} )  (g(y_i)^{1-\delta_i} G(y_i^+)^{\delta_i})
\]

Only keep the terms involving $\theta$:  
\[
L(\theta)= \prod_{i=1}^n(f(y_i; \theta)^{\delta_i} S(y_i; \theta)^{1-\delta_i})
\]

---

## 5. An example of Exponential distribution

Suppose $T\sim exp(\theta)$, $C\perp T$.
\[
L(\theta)=\prod_{i=1}^n(\theta^{\delta_i} e^{-\theta y_i})
\]

\[
\log L(\theta)=\sum_{i=1}^n(\delta_i \log \theta - \theta y_i)
\]

\[
U(\theta)=\frac{d}{d\theta}\log L(\theta)=\frac{\sum_{i=1}^n \delta_i}{\theta}-\sum_{i=1}^n y_i
\]

\[
\Rightarrow \hat{\theta}=\frac{\sum_{i=1}^n\delta_i}{\sum_{i=1}^n y_i}
\]
